access the payload of a vldata

src/lowparse/LowParse.Low.VLData.fst
@@ -454,7 +454,7 @@ let valid_bounded_vldata_strong_intro
   valid_bounded_vldata_intro h min max p input pos pos'
 
 inline_for_extraction
-let finalize_bounded_vldata_strong
+let finalize_bounded_vldata_strong_exact
   (min: nat)
   (max: nat { min <= max /\ max > 0 /\ max < 4294967296 } )
   (#k: parser_kind)
@@ -489,7 +489,44 @@ let finalize_bounded_vldata_strong
   valid_bounded_vldata_strong_intro h min max s input pos pos'
 
 inline_for_extraction
-let weak_finalize_bounded_vldata_strong
+let finalize_bounded_vldata_strong
+  (min: nat)
+  (max: nat { min <= max /\ max > 0 /\ max < 4294967296 } )
+  (#k: parser_kind)
+  (#t: Type0)
+  (#p: parser k t)
+  (s: serializer p)
+  (input: slice)
+  (pos: U32.t)
+  (pos' : U32.t)
+: HST.Stack unit
+  (requires (fun h ->
+    let sz = log256' max in
+    U32.v pos + sz <= U32.v input.len /\ (
+    let pos_payload = pos `U32.add` U32.uint_to_t sz in
+    valid_pos p h input pos_payload pos' /\
+    k.parser_kind_subkind == Some ParserStrong /\ (
+    let len_payload = pos' `U32.sub` pos_payload in
+    min <= U32.v len_payload /\ U32.v len_payload <= max
+  ))))
+  (ensures (fun h _ h' ->
+    let sz = log256' max in
+    let x = contents p h input (pos `U32.add` U32.uint_to_t sz) in
+    B.modifies (loc_slice_from_to input pos (pos `U32.add` U32.uint_to_t sz)) h h' /\
+    parse_bounded_vldata_strong_pred min max s x /\
+    valid_content_pos (parse_bounded_vldata_strong min max s) h' input pos x pos'
+  ))
+= let h = HST.get () in
+  [@inline_let]
+  let _ =
+    let sz = log256' max in
+    let pos_payload = pos `U32.add` U32.uint_to_t sz in
+    valid_pos_valid_exact p h input pos_payload pos'
+  in
+  finalize_bounded_vldata_strong_exact min max s input pos pos'
+  
+inline_for_extraction
+let weak_finalize_bounded_vldata_strong_exact
   (min: nat)
   (max: nat { min <= max /\ max > 0 /\ max < 4294967296 } )
   (#k: parser_kind)
@@ -523,48 +560,128 @@ let weak_finalize_bounded_vldata_strong
   if U32.uint_to_t max `U32.lt` len_payload || len_payload `U32.lt` U32.uint_to_t min
   then false
   else begin
-    finalize_bounded_vldata_strong min max s input pos pos';
+    finalize_bounded_vldata_strong_exact min max s input pos pos';
     true
   end
 
-(*
-#set-options "--z3rlimit 64"
-
 inline_for_extraction
-let accessor_bounded_vldata_payload
+let weak_finalize_bounded_vldata_strong
   (min: nat)
-  (max: nat)
-  (#k: parser_kind)
-  (#t: Type0)
-  (p: parser k t)
-  (sz32: U32.t)
-  (u: unit {
-    min <= max /\ max > 0 /\ max < 4294967296 /\
-    U32.v sz32 == log256' max
-  })
-: Tot (accessor (parse_bounded_vldata min max p) p (fun x y -> y == x))
-= [@inline_let]
-  let sz = log256' max in
-  fun input ->
-  let h = HST.get () in
-  parse_bounded_vldata_elim_forall min max p (B.as_seq h input);
-  let len = read_bounded_integer sz input in
-  B.sub (B.offset input sz32) 0ul len
-
-inline_for_extraction
-let accessor_bounded_vldata_strong_payload
-  (min: nat)
-  (max: nat)
+  (max: nat { min <= max /\ max > 0 /\ max < 4294967296 } )
   (#k: parser_kind)
   (#t: Type0)
   (#p: parser k t)
   (s: serializer p)
-  (sz32: U32.t)
-  (u: unit {
-    min <= max /\ max > 0 /\ max < 4294967296 /\
-    U32.v sz32 == log256' max
-  })
-: Tot (accessor (parse_bounded_vldata_strong min max s) p (fun x y -> y == x))
-= fun input -> accessor_bounded_vldata_payload min max p sz32 () input
+  (input: slice)
+  (pos: U32.t)
+  (pos' : U32.t)
+: HST.Stack bool
+  (requires (fun h ->
+    let sz = log256' max in
+    U32.v pos + sz <= U32.v input.len /\
+    k.parser_kind_subkind == Some ParserStrong /\ (
+    let pos_payload = pos `U32.add` U32.uint_to_t sz in
+    valid_pos p h input pos_payload pos'
+  )))
+  (ensures (fun h res h' ->
+    let sz = log256' max in
+    let pos_payload = pos `U32.add` U32.uint_to_t sz in
+    let len_payload = pos' `U32.sub` pos_payload in
+    B.modifies (loc_slice_from_to input pos (pos `U32.add` U32.uint_to_t sz)) h h' /\
+    (res == true <==> (min <= U32.v len_payload /\ U32.v len_payload <= max)) /\
+    (if res
+    then
+      let x = contents p h input pos_payload in
+      parse_bounded_vldata_strong_pred min max s x /\
+      valid_content_pos (parse_bounded_vldata_strong min max s) h' input pos x pos'
+    else True
+  )))
+= let h = HST.get () in
+  [@inline_let]
+  let _ =
+    let sz = log256' max in
+    let pos_payload = pos `U32.add` U32.uint_to_t sz in
+    valid_pos_valid_exact p h input pos_payload pos'
+  in
+  weak_finalize_bounded_vldata_strong_exact min max s input pos pos'
 
-#reset-options
+
+#push-options "--z3rlimit 16"
+
+let gaccessor_bounded_vldata_payload
+  (min: nat)
+  (max: nat { min <= max /\ max > 0 /\ max < 4294967296 } )
+  (#k: parser_kind)
+  (#t: Type0)
+  (p: parser k t)
+: Tot (gaccessor (parse_bounded_vldata min max p) p (clens_id t))
+= fun input ->
+  let sz = log256' max in
+  parse_vldata_gen_eq sz (in_bounds min max) p input;
+  let res =
+    if Seq.length input < sz
+    then (assert (None? (parse (parse_bounded_integer sz) input)); (0, 0)) // dummy
+    else begin
+      assert (Some? (parse (parse_bounded_integer sz) input));
+      let Some (_, consumed) = parse (parse_bounded_integer sz) input in
+      assert (consumed == sz);
+      (sz, Seq.length input - sz)
+    end
+  in
+  (res <: (res : _ { gaccessor_post' (parse_bounded_vldata min max p) p (clens_id _) input res } ))
+
+#pop-options
+
+inline_for_extraction
+let accessor_bounded_vldata_payload
+  (min: nat)
+  (max: nat { min <= max /\ max > 0 /\ max < 4294967296 } )
+  (#k: parser_kind)
+  (#t: Type0)
+  (p: parser k t)
+: Tot (accessor (gaccessor_bounded_vldata_payload min max p))
+= fun input pos ->
+  let h = HST.get () in
+  [@inline_let]
+  let _ = slice_access_eq h (gaccessor_bounded_vldata_payload min max p) input pos in
+  pos `U32.add` U32.uint_to_t (log256' max)
+
+
+let clens_bounded_vldata_strong_payload
+  (min: nat)
+  (max: nat { min <= max /\ max > 0 /\ max < 4294967296 } )
+  (#k: parser_kind)
+  (#t: Type0)
+  (#p: parser k t)
+  (s: serializer p)
+: Tot (clens (parse_bounded_vldata_strong_t min max s) t)
+= {
+  clens_cond = (fun _ -> True);
+  clens_get = (fun (x: parse_bounded_vldata_strong_t min max s) -> (x <: t));
+}
+
+let gaccessor_bounded_vldata_strong_payload
+  (min: nat)
+  (max: nat { min <= max /\ max > 0 /\ max < 4294967296 } )
+  (#k: parser_kind)
+  (#t: Type0)
+  (#p: parser k t)
+  (s: serializer p)
+: Tot (gaccessor (parse_bounded_vldata_strong min max s) p (clens_bounded_vldata_strong_payload min max s))
+= fun input ->
+  (gaccessor_bounded_vldata_payload min max p input <: (res : _ { gaccessor_post' (parse_bounded_vldata_strong min max s) p (clens_bounded_vldata_strong_payload min max s) input res } ))
+
+inline_for_extraction
+let accessor_bounded_vldata_strong_payload
+  (min: nat)
+  (max: nat { min <= max /\ max > 0 /\ max < 4294967296 } )
+  (#k: parser_kind)
+  (#t: Type0)
+  (#p: parser k t)
+  (s: serializer p)
+: Tot (accessor (gaccessor_bounded_vldata_strong_payload min max s))
+= fun input pos ->
+  let h = HST.get () in
+  [@inline_let]
+  let _ = slice_access_eq h (gaccessor_bounded_vldata_strong_payload min max s) input pos in
+  pos `U32.add` U32.uint_to_t (log256' max)
